# imports: http://purl.obolibrary.org/obo/bfo/2020/bfo-core.ttl
# imports: https://ontology.unifiedcyberontology.org/uco/uco/1.3.0

@prefix drafting: <http://example.org/ontology/drafting/> .
@prefix obo: <http://purl.obolibrary.org/obo/> .
@prefix owl: <http://www.w3.org/2002/07/owl#> .
@prefix rdf: <http://www.w3.org/1999/02/22-rdf-syntax-ns#> .
@prefix rdfs: <http://www.w3.org/2000/01/rdf-schema#> .
@prefix uco-action: <https://ontology.unifiedcyberontology.org/uco/action/> .
@prefix uco-core: <https://ontology.unifiedcyberontology.org/uco/core/> .
@prefix uco-identity: <https://ontology.unifiedcyberontology.org/uco/identity/> .
@prefix uco-location: <https://ontology.unifiedcyberontology.org/uco/location/> .
@prefix uco-observable: <https://ontology.unifiedcyberontology.org/uco/observable/> .
@prefix uco-pattern: <https://ontology.unifiedcyberontology.org/uco/pattern/> .
@prefix uco-role: <https://ontology.unifiedcyberontology.org/uco/role/> .
@prefix xsd: <http://www.w3.org/2001/XMLSchema#> .

<http://example.org/ontology/uco-bfo>
	a owl:Ontology ;
	owl:imports
		<http://purl.obolibrary.org/obo/bfo/2020/bfo-core.ttl> ,
		<https://ontology.unifiedcyberontology.org/uco/uco/1.3.0>
		;
	.

drafting:Endurant
	a owl:Class ;
	rdfs:subClassOf
		obo:BFO_0000002 ,
		uco-core:UcoThing
		;
	rdfs:isDefinedBy <https://github.com/ucoProject/UCO/issues/544> ;
	owl:disjointWith drafting:Perdurant ;
	.

drafting:Perdurant
	a owl:Class ;
	rdfs:subClassOf
		obo:BFO_0000003 ,
		uco-core:UcoObject
		;
	rdfs:isDefinedBy <https://github.com/ucoProject/UCO/issues/544> ;
	owl:disjointWith drafting:Endurant ;
	.

drafting:Quality
	a owl:Class ;
	rdfs:subClassOf
		drafting:Endurant ,
		obo:BFO_0000019 ,
		uco-core:UcoInherentCharacterizationThing
		;
	.

uco-action:Action
	rdfs:subClassOf
		drafting:Perdurant ,
		obo:BFO_0000015
		;
	.

uco-core:Event
	rdfs:subClassOf
		drafting:Perdurant ,
		obo:BFO_0000008
		;
	.

uco-core:Facet
	rdfs:subClassOf obo:BFO_0000020 ;
	.

uco-core:Item
	rdfs:subClassOf drafting:Endurant ;
	.

uco-core:hasFacet
	rdfs:subPropertyOf obo:BFO_0000196 ;
	.

uco-identity:Identity
	rdfs:subClassOf drafting:Endurant ;
	.

uco-identity:Person
	rdfs:subClassOf obo:BFO_0000040 ;
	.

uco-location:Location
	rdfs:subClassOf
		drafting:Endurant ,
		obo:BFO_0000006
		;
	.

uco-observable:ContentData
	rdfs:subClassOf obo:BFO_0000004 ;
	.

uco-observable:Device
	rdfs:subClassOf obo:BFO_0000040 ;
	.

uco-observable:File
	rdfs:subClassOf obo:BFO_0000031 ;
	.

uco-observable:ObservablePattern
	rdfs:subClassOf drafting:Endurant ;
	.

uco-pattern:LogicalPattern
	rdfs:subClassOf drafting:Endurant ;
	.

[]
	a owl:Axiom ;
	rdfs:comment "Note that BFO 196 ('bearer of') has a domain restriction, that the subject not be a spatial region.  This could cause conflicts with UCO's Location namespace: If uco-location:Location or some subclass are believed to be specializations of BFO 6 ('spatial region'), then with this alignment of BFO 196, they cannot have a Facet."@en ;
	owl:annoatedProperty rdfs:subPropertyOf ;
	owl:annotatedObject obo:BFO_0000196 ;
	owl:annotatedSubject uco-core:hasFacet ;
	.

[]
	a owl:Axiom ;
	rdfs:comment "Per an example of usage from BFO 2.0, 'the pdf file on your laptop, the pdf file that is a copy thereof on my laptop'."@en ;
	owl:annotatedProperty rdfs:subClassOf ;
	owl:annotatedSource uco-observable:File ;
	owl:annotatedTarget obo:BFO_0000031 ;
	.

[]
	a owl:Axiom ;
	rdfs:comment "Per usage with a Quality that presents a ContentData object's ability to be measured with the result being a Hash.  This usage with BFO_0000080 requires the quality-bearer be an independent continuant, but does not require a more specific subclass."@en ;
	owl:annotatedProperty rdfs:subClassOf ;
	owl:annotatedSource uco-observable:ContentData ;
	owl:annotatedTarget obo:BFO_0000004 ;
	.

